# 时域离散信号和时域离散系统-第一章习题 - 提交版本

姓名：孙武周
学号：2021113501
# Question 3:
![](../../attachments/Pasted%20image%2020240922184822.png)

(1) 
solution: the expression is the Sinusoidal sequence, we can compute $T$ as follow:
$T=\frac{2*\pi}{\frac{3*\pi}{7}}=\frac{14}{3}$
the $\frac{14}{3}$ is a rational number but not interger number, we can get the $T=14$, so the $x(n)$ **is periodic sequence**.

(2)
solution：coz the expresion $x(n)=e^{j*(\frac{1}{8}*n-\pi)}=e^{j*\frac{n}{8}-j*\pi}$, we can find the $\sigma=-\pi$ , but this don't make difference on the $T$. so we can change the expression into $x(n)=cos(\omega_0 *n)+j*sin(\omega_0 *n)$ . Then we can compute the $T$ as follow:
$T=\frac{2*\pi}{\frac{1}{8}}=16\pi$
because the $16\pi$ is  **irrational number** , so the $x(n)$ **is not periodic sequence**.


# Question 5
![](../../attachments/Pasted%20image%2020240922193133.png)

(5)
solution: 
first step : prove if the system is linear 
$y_1(n)=T[x_1(n)]=x_1^2(n)$ 
$y_2(n)=T[x_2(n)]=x_2^2(n)$
$y(n)=T[a*x_1(n)+b*x_2(n)]=(a*x_1(n)+b*x_2(n))^2 \ne a*y_1(n)+b*y_2(n)$
the equation $y(n)=x^2(n)$ is not linear.

second step: prove if the system is time invariance
$y(n)=x^2(n)$
$y(n-n_0)=x^2(n-n_0)$
$T[x(n-n_0)]=x^2(n-n_0)$
coz the $T[x(n-n_0)]=y(n-n_0)$
so the equation is time invariance.

therefore, the equation **is not linear and time invariance.**

(6)
solution:
first step : prove if the system is linear 
$y_1(n)=T[x_1(n)]=x_1(n^2)$ 
$y_2(n)=T[x_2(n)]=x_2(n^2)$
$y(n)=T[a*x_1(n)+b*x_2(n)]=a*x_1(n^2)+b*x_2(n^2)=a*y_1+b*y_2$
the equation $y(n)=x(n^2)$ is  linear.

second step: prove if the system is time invariance
$y(n)=x(n^2)$
$y(n-n_0)=x(n-n_0)^2$
$T[x(n-n_0)]=x(n-n_0)^2$

because the $T[x(n-n_0)]=y(n-n_0)$, so the equation is time invariance.

therefore, the equation **is linear and time invariance**.

(7)
solution:
first step: prove if the sytem $y(n)=\sum_{m=0}^n x(m)$ is linear
$y_1(n)=T[x_1(n)]=\sum_{m=0}^n x_1(m)$
$y_2(n)=T[x_2(n)]=\sum_{m=0}^n x_2(m)$
$y(n)=T[a*x_1(n)+b*x_2(n)]=\sum_{m=0}^n (a*x_1(m)+b*x_2(m))=a*\sum_{m=0}^n x_1(m)+b*\sum_{m=0}^n x_2(m)=a*y_1(n)+b*y_2(n)$

second step: prove if the sytem $y(n)=\sum_{m=0}^n x(m)$ is time invariance
$y(n-n_0)=\sum_{m=0}^{n-n_0}x(m) \ne T[x(n-n_0)]=\sum_{m=0}^n x(n-n_0)$
the sytem $y(n)=\sum_{m=0}^n x(m)$ is not time invariance

therefor, the system **is  linear and not time invariance.**
(8)
solution:
first step: prove if the system $y(n)=x(n)sin(\omega *n)$
$y_1(n)=T[x_1(n)]=x_1(n)sin(\omega *n)$
$y_2(n)=T[x_2(n)]=x_2(n)sin(\omega *n)$
$y_n(n)=T[a*x_1(n)+b*x_2(n)]=(a*x_1(n)+b*x_2(n))sin(\omega *n)=a*y_1+b*y_2$
so this system is linear.

second step: prove if this system if time invariance
$y(n-n_0)=x(n-n0)sin(\omega *(n-n0))$
$T[x(n-n_0)]=x(n-n0)sin(\omega *n)$
$y(n-n_0) \ne T[x(n-n_0)]$
so this system is not time invarance 

so this system is **linear and not time invarance.**

# Question 6
![](../../attachments/Pasted%20image%2020240922211404.png)

(3)
solution:
$y=\sum_{k=n-n_0}^{n+n_0}x(k)$ is causal and stable system when $n_0=0$. 

$y=\sum_{k=n-n_0}^{n+n_0}x(k)$ is not causal but stable system when $n_0 \ne 0$. 


The proof is follow:
first step: prove if it's the casual system
if $n_0=0$, this system is casual system because y is only dependent on n
if $n_0 \ne 0$, this system is not casual system because y is also dependent on the variable bigger than n, not only n or smaller than n. 

second step: prove if it's the stable system
Then we assume the $|x(n)|<A$, the $|y|<(2n_0+1)A$, so this system have the limit bound. We can conclude this system is stable system.

(4)
solution:
$y(n)=x(n-n_0)$ is casual stable system when the $n_0 \ge 0$ 

$y(n)=x(n-n_0)$ is not casual but stable system when the $n_0 < 0$ 


first step: prove if it's casual system.
if $n_0<0$, the y will be dependent on the variable bigger than n.
if $n_0 \ge 0$, the y is only dependent on the n and the variable smaller than n.  

second step:
let us assume the $|x(n)| \le A$, the $|y|<A$, so the output has limit bound with the input limit bound. Then we conclude this system is stable system.

# Question 8
![](../../attachments/Pasted%20image%2020240922221321.png)
(3)
$y(n)=x(n)*h(n)=\sum_{m=-\infty}^{\infty}x(m)h(n-m)=\sum_{m=-\infty}^{\infty}R_5(m)0.5^n u(n-m)$, the $*$ here means the conv

when the $0 \le m \le 4$, the value of $R_5(m)$  is non-zero.
when the $n \le m$, the value of $u(n-m)$ is non-zero.
so, we need to satisfy the two equation to compute the sum of $\sum_{m=-\infty}^{\infty}R_5(m)0.5^n u(n-m)$

when the $n<0$, $y(n)=0$
when the $0 \le n \le 4$, $y(n)=\sum_{m=0}^n {0.5}^{n-m}={0.5}^n\frac{1-{0.5}^{-n-1}}{1-{0.5}^{-1}}=2-{0.5}^n$
when the $n \ge 5$, $y(n)=31*0.5^n$, the * here means multy.

# Question 11
![](../../attachments/Pasted%20image%2020240922221427.png)


let us assume the $x(n)=\sigma(n)$, then $h(n)=\frac{1}{2}h(n-1)+\sigma(n) +\frac{1}{2} \sigma(n-1)$
when $n=0$, the $h(0)=\frac{1}{2}h(-1)+\sigma(0) +\frac{1}{2}\sigma(-1)=1$
when $n=1$, the $h(1)=\frac{1}{2}h(0)+\sigma(1) +\frac{1}{2}\sigma(0)=1$
when $n=2$, the $h(2)=\frac{1}{2}h(1)=\frac{1}{2}$
when $n=3$, the $h(3)=\frac{1}{2}h(2)=(\frac{1}{2})^2$
therefore, we can conclude the $h(n)=(\frac{1}{2})^{n-1}u(n-1)+\sigma(n)$
